reorganizing

proof/correctness/avx2/MLKEM_genmatrix_avx2.ec
@@ -1,9 +1,9 @@
-require import AllCore IntDiv.
+require import AllCore IntDiv List.
 from Jasmin require import JModel.
 
 require import Array16 Array25 Array32 Array33 Array128 Array136 Array256 Array768 Array960 Array1024 Array1088 Array2304.
 
-require import MLKEM_InnerPKE NTT_avx2 MLKEMFCLib.
+require import MLKEM_InnerPKE NTT_avx2 MLKEMFCLib AVX2_Ops NTT_AVX_Fq MLKEM_Poly_avx2_vec.
 
 import NTT_Avx2.
 
@@ -12,6 +12,254 @@ require import Jkem_avx2 Jkem.
 import GFq Rq Sampling Serialization Symmetric VecMat InnerPKE MLKEM Fq Correctness.
 import PolyMat.
 import KMatrix.Matrix.
+import MLKEM_PolyAVXVec.
+import WArray136 WArray32 WArray128.
+import WArray512 WArray256.
+
+
+(********* MOVED HERE TO AVOID CIRCULAR DEPS ************)
+
+(* move somewhere else *)
+
+lemma prod (x:'a*'b) :
+ x = (x.`1,x.`2). smt(). qed.
+
+lemma bits8_W32u8 ws i :
+  W32u8.pack32_t ws \bits8 i = if 0 <= i < 32 then ws.[i] else W8.zero.
+apply W8.wordP => j hj.
+case (0 <= i < 32) => hi. rewrite  W32u8.pack32bE //. rewrite get_out //. qed.
+
+lemma ianda a b c : a => (b => c) => ((a => b) => c). smt(). qed.
+
+lemma if_eq (a:bool) (b c d:'a) : (a => (b=d)) => (!a => (c=d)) => (if a then b else c) = d.
+move => T F. case a => />. qed.
+
+
+lemma rng_iotared i n :
+  (0 <= i < n) = (i \in iotared 0 n).
+rewrite iotaredE mem_iota //= andaE //. qed.
+
+op pack16x8 (x:('a Array16.t)*('a Array16.t)*('a Array16.t)*('a Array16.t)*('a Array16.t)*('a Array16.t)*('a Array16.t)*('a Array16.t)) : 'a Array128.t = Array128.init (fun i =>
+ if 0 <= i < 16 then x.`1.[i%%16]
+ else if 16 <= i < 32 then x.`2.[i%%16]
+ else if 32 <= i < 48 then x.`3.[i%%16]
+ else if 48 <= i < 64 then x.`4.[i%%16]
+ else if 64 <= i < 80 then x.`5.[i%%16]
+ else if 80 <= i < 96 then x.`6.[i%%16]
+ else if 96 <= i < 112 then x.`7.[i%%16]
+ else x.`8.[i%%16]) axiomatized by pack16x8E.
+
+op unpack16x8 (x:'a Array128.t) : ('a Array16.t)*('a Array16.t)*('a Array16.t)*('a Array16.t)*('a Array16.t)*('a Array16.t)*('a Array16.t)*('a Array16.t) =
+ (Array16.init (fun i => x.[i+16*0])
+ ,Array16.init (fun i => x.[i+16*1])
+ ,Array16.init (fun i => x.[i+16*2])
+ ,Array16.init (fun i => x.[i+16*3])
+ ,Array16.init (fun i => x.[i+16*4])
+ ,Array16.init (fun i => x.[i+16*5])
+ ,Array16.init (fun i => x.[i+16*6])
+ ,Array16.init (fun i => x.[i+16*7])) axiomatized by unpack16x8E.
+
+lemma unpack16x8K (w:'a Array128.t) :
+  pack16x8 (unpack16x8 w) = w.
+rewrite pack16x8E unpack16x8E tP => i Hi. rewrite !initiE //=. rewrite !initiE //= 1..8:/#.
+smt(). qed.
+
+lemma pack16x8K (w:('a Array16.t)*('a Array16.t)*('a Array16.t)*('a Array16.t)*('a Array16.t)*('a Array16.t)*('a Array16.t)*('a Array16.t)) :
+  unpack16x8 (pack16x8 w) = w.
+rewrite pack16x8E unpack16x8E => />. rewrite (_:w=(w.`1,w.`2,w.`3,w.`4,w.`5,w.`6,w.`7,w.`8)) => />. smt(). progress.
+rewrite tP => i Hi. rewrite !initiE //= /#. 
+rewrite tP => i Hi; rewrite !initiE //= !initiE //= /#.
+rewrite tP => i Hi. rewrite !initiE //= !initiE //= /#. 
+rewrite tP => i Hi. rewrite !initiE //= !initiE //= /#. 
+rewrite tP => i Hi. rewrite !initiE //= !initiE //= /#. 
+rewrite tP => i Hi. rewrite !initiE //= !initiE //= /#.
+rewrite tP => i Hi. rewrite !initiE //= !initiE //= /#.
+rewrite tP => i Hi. rewrite !initiE //= !initiE //= /#.
+qed.
+
+op pack128x2 (x:'a Array128.t * 'a Array128.t) : 'a Array256.t = Array256.init (fun i =>
+  if 0 <= i < 128 then x.`1.[i%%128]
+  else x.`2.[i%%128]) axiomatized by pack128x2E.
+
+op unpack128x2 (x:'a Array256.t) : ('a Array128.t * 'a Array128.t) =
+ (Array128.init (fun i => x.[i+128*0])
+ ,Array128.init (fun i => x.[i+128*1])) axiomatized by unpack128x2E.
+
+lemma unpack128x2K (w:'a Array256.t) :
+  pack128x2 (unpack128x2 w) = w.
+rewrite pack128x2E unpack128x2E tP => i Hi. rewrite !initiE //=. rewrite !initiE //= 1..2:/#.
+smt(). qed.
+
+lemma pack128x2K (w:('a Array128.t)*('a Array128.t)) :
+  unpack128x2 (pack128x2 w) = w.
+rewrite pack128x2E unpack128x2E => />. rewrite (_:w=(w.`1,w.`2)) => />. smt(). progress.
+rewrite tP => i Hi. rewrite !initiE //= /#. 
+rewrite tP => i Hi. rewrite !initiE //= !initiE //= /#. 
+qed.
+
+abbrev is16u16x8 (x:t16u16*t16u16*t16u16*t16u16*t16u16*t16u16*t16u16*t16u16) (y:vt16u16*vt16u16*vt16u16*vt16u16*vt16u16*vt16u16*vt16u16*vt16u16) = is16u16 x.`1 y.`1 /\ is16u16 x.`2 y.`2 /\ is16u16 x.`3 y.`3 /\ is16u16 x.`4 y.`4 /\ is16u16 x.`5 y.`5 /\ is16u16 x.`6 y.`6 /\ is16u16 x.`7 y.`7 /\ is16u16 x.`8 y.`8.
+
+abbrev nttunpack128x16 ['a] (x:('a Array16.t)*('a Array16.t)*('a Array16.t)*('a Array16.t)*('a Array16.t)*('a Array16.t)*('a Array16.t)*('a Array16.t)) = unpack16x8 (nttunpack128 (pack16x8 x)).
+
+lemma rng_perm_nttunpack128 i :
+  0 <= i < 128 => 
+  0 <= nth witness perm_nttunpack128 i < 128.
+move => *. rewrite perm_nttunpack128E => />. smt(). qed.
+
+lemma nttunpack128x2 (w:'a Array256.t) :
+  unpack128x2 (nttunpack w) = (nttunpack128 (unpack128x2 w).`1,nttunpack128 (unpack128x2 w).`2).
+rewrite !unpack128x2E /nttunpack128 //=. split.
++ rewrite tP => i Hi. rewrite !initiE //=. rewrite !initiE //=. rewrite rng_perm_nttunpack128 //.
+rewrite /nttunpack /perm_nttunpack128 initiE //= 1:/#.
+move:Hi. rewrite rng_iotared => />. do 128!(try (move => Hi; case Hi => />)). 
++ rewrite tP => i Hi. rewrite !initiE //=. rewrite !initiE //=. rewrite rng_perm_nttunpack128 //.
+rewrite /nttunpack /perm_nttunpack128 initiE //= 1:/#.
+move:Hi. rewrite rng_iotared => />. do 128!(try (move => Hi; case Hi => />)). 
+qed.
+
+lemma inj_unpack16x8 (x y : 'a Array128.t) :
+  (unpack16x8 x = unpack16x8 y) => (x = y).
+rewrite -(unpack16x8K x) -(unpack16x8K y). rewrite !pack16x8K => ->. rewrite unpack16x8K //. qed.
+
+lemma inj_unpack128x2 (x y : 'a Array256.t) :
+  (unpack128x2 x = unpack128x2 y) => (x = y).
+rewrite -(unpack128x2K x) -(unpack128x2K y). rewrite !pack128x2K => ->. rewrite unpack128x2K //. qed.
+
+lemma nttunpack128_corr_h a :
+ hoare[ Jkem_avx2.M(Jkem_avx2.Syscall).__nttunpack128 :
+   is16u16x8 a arg ==> is16u16x8 (nttunpack128x16 a) res].
+proc.
+(*shuffle8*)
+pose r0_8 := (shuf8 a.`1 a.`5).`1.
+pose r1_8 := (shuf8 a.`2 a.`6).`1.
+pose r2_8 := (shuf8 a.`3 a.`7).`1.
+pose r3_8 := (shuf8 a.`4 a.`8).`1.
+pose r4_8 := (shuf8 a.`1 a.`5).`2.
+pose r5_8 := (shuf8 a.`2 a.`6).`2.
+pose r6_8 := (shuf8 a.`3 a.`7).`2.
+pose r7_8 := (shuf8 a.`4 a.`8).`2.
+seq 1 : (is16u16x8 (r0_8,a.`2,a.`3,a.`4,r4_8,a.`6,a.`7,a.`8) (r0,r1,r2,r3,r4,r5,r6,r7)). auto => />. call (avx2_shuffle8_corr_h a.`1 a.`5) => />. auto => />. 
+seq 1 : (is16u16x8 (r0_8,r1_8,a.`3,a.`4,r4_8,r5_8,a.`7,a.`8) (r0,r1,r2,r3,r4,r5,r6,r7)). auto => />. call (avx2_shuffle8_corr_h a.`2 a.`6) => />. auto => />.
+seq 1 : (is16u16x8 (r0_8,r1_8,r2_8,a.`4,r4_8,r5_8,r6_8,a.`8) (r0,r1,r2,r3,r4,r5,r6,r7)). auto => />. call (avx2_shuffle8_corr_h a.`3 a.`7) => />. auto => />.
+seq 1 : (is16u16x8 (r0_8,r1_8,r2_8,r3_8,r4_8,r5_8,r6_8,r7_8) (r0,r1,r2,r3,r4,r5,r6,r7)). auto => />. call (avx2_shuffle8_corr_h a.`4 a.`8) => />. auto => />.
+(*shuffle4*)
+pose r0_4 := (shuf4 r0_8 r2_8).`1.
+pose r1_4 := (shuf4 r1_8 r3_8).`1.
+pose r2_4 := (shuf4 r0_8 r2_8).`2.
+pose r3_4 := (shuf4 r1_8 r3_8).`2.
+pose r4_4 := (shuf4 r4_8 r6_8).`1.
+pose r5_4 := (shuf4 r5_8 r7_8).`1.
+pose r6_4 := (shuf4 r4_8 r6_8).`2.
+pose r7_4 := (shuf4 r5_8 r7_8).`2.
+seq 1 : (is16u16x8 (r0_4,r1_8,r2_4,r3_8,r4_8,r5_8,r6_8,r7_8) (r0,r1,r2,r3,r4,r5,r6,r7)). auto => />. call (avx2_shuffle4_corr_h r0_8 r2_8) => />. auto => />.
+seq 1 : (is16u16x8 (r0_4,r1_8,r2_4,r3_8,r4_4,r5_8,r6_4,r7_8) (r0,r1,r2,r3,r4,r5,r6,r7)). auto => />. call (avx2_shuffle4_corr_h r4_8 r6_8) => />. auto => />.
+seq 1 : (is16u16x8 (r0_4,r1_4,r2_4,r3_4,r4_4,r5_8,r6_4,r7_8) (r0,r1,r2,r3,r4,r5,r6,r7)). auto => />. call (avx2_shuffle4_corr_h r1_8 r3_8) => />. auto => />.
+seq 1 : (is16u16x8 (r0_4,r1_4,r2_4,r3_4,r4_4,r5_4,r6_4,r7_4) (r0,r1,r2,r3,r4,r5,r6,r7)). auto => />. call (avx2_shuffle4_corr_h r5_8 r7_8) => />. auto => />.
+(*shuffle2*)
+pose r0_2 := (shuf2 r0_4 r1_4).`1.
+pose r1_2 := (shuf2 r0_4 r1_4).`2.
+pose r2_2 := (shuf2 r2_4 r3_4).`1.
+pose r3_2 := (shuf2 r2_4 r3_4).`2.
+pose r4_2 := (shuf2 r4_4 r5_4).`1.
+pose r5_2 := (shuf2 r4_4 r5_4).`2.
+pose r6_2 := (shuf2 r6_4 r7_4).`1.
+pose r7_2 := (shuf2 r6_4 r7_4).`2.
+seq 1 : (is16u16x8 (r0_2,r1_2,r2_4,r3_4,r4_4,r5_4,r6_4,r7_4) (r0,r1,r2,r3,r4,r5,r6,r7)). auto => />. call (avx2_shuffle2_corr_h r0_4 r1_4) => />. auto => />.
+seq 1 : (is16u16x8 (r0_2,r1_2,r2_2,r3_2,r4_4,r5_4,r6_4,r7_4) (r0,r1,r2,r3,r4,r5,r6,r7)). auto => />. call (avx2_shuffle2_corr_h r2_4 r3_4) => />. auto => />.
+seq 1 : (is16u16x8 (r0_2,r1_2,r2_2,r3_2,r4_2,r5_2,r6_4,r7_4) (r0,r1,r2,r3,r4,r5,r6,r7)). auto => />. call (avx2_shuffle2_corr_h r4_4 r5_4) => />. auto => />.
+seq 1 : (is16u16x8 (r0_2,r1_2,r2_2,r3_2,r4_2,r5_2,r6_2,r7_2) (r0,r1,r2,r3,r4,r5,r6,r7)). auto => />. call (avx2_shuffle2_corr_h r6_4 r7_4) => />. auto => />.
+(*shuffle1*)
+pose r0_1 := (shuf1 r0_2 r4_2).`1.
+pose r1_1 := (shuf1 r1_2 r5_2).`1.
+pose r2_1 := (shuf1 r2_2 r6_2).`1.
+pose r3_1 := (shuf1 r3_2 r7_2).`1.
+pose r4_1 := (shuf1 r0_2 r4_2).`2.
+pose r5_1 := (shuf1 r1_2 r5_2).`2.
+pose r6_1 := (shuf1 r2_2 r6_2).`2.
+pose r7_1 := (shuf1 r3_2 r7_2).`2.
+seq 1 : (is16u16x8 (r0_1,r1_2,r2_2,r3_2,r4_1,r5_2,r6_2,r7_2) (r0,r1,r2,r3,r4,r5,r6,r7)). auto => />. call (avx2_shuffle1_corr_h r0_2 r4_2) => />. auto => />.
+seq 1 : (is16u16x8 (r0_1,r1_1,r2_2,r3_2,r4_1,r5_1,r6_2,r7_2) (r0,r1,r2,r3,r4,r5,r6,r7)). auto => />. call (avx2_shuffle1_corr_h r1_2 r5_2) => />. auto => />.
+seq 1 : (is16u16x8 (r0_1,r1_1,r2_1,r3_2,r4_1,r5_1,r6_1,r7_2) (r0,r1,r2,r3,r4,r5,r6,r7)). auto => />. call (avx2_shuffle1_corr_h r2_2 r6_2) => />. auto => />.
+seq 1 : (is16u16x8 (r0_1,r1_1,r2_1,r3_1,r4_1,r5_1,r6_1,r7_1) (r0,r1,r2,r3,r4,r5,r6,r7)). auto => />. call (avx2_shuffle1_corr_h r3_2 r7_2) => />. auto => />.
+(*end*)
+auto => /> &m -> -> -> -> -> -> -> ->. 
+do 8!(try split; first by
+ apply W16u16.wordP => i Hi; rewrite !bits16_W16u16 // Hi //= !of_listE !list_arr16 !initiE //=; rewrite /to_list !nth_mkseq //=; move:Hi; rewrite rng_iotared => />;
+ do 16!(try(move => Hi; case Hi => />); first by rewrite /nttunpack128 /perm_nttunpack128 unpack16x8E pack16x8E => />)).
+qed.
+
+lemma __nttunpack128_ll: islossless Jkem_avx2.M(Jkem_avx2.Syscall).__nttunpack128 by islossless.
+
+phoare nttunpack128_corr a :
+ [ Jkem_avx2.M(Jkem_avx2.Syscall).__nttunpack128 :
+   is16u16x8 a arg ==> is16u16x8 (nttunpack128x16 a) res] = 1%r.
+conseq __nttunpack128_ll (nttunpack128_corr_h a) => />. qed.
+
+lemma nttunpack_corr_h a :
+ hoare[ Jkem_avx2.M(Jkem_avx2.Syscall)._nttunpack : arg = a ==> res = nttunpack a].
+proc. sp. 
+seq 1 : (rp=a /\ is16u16x8 (nttunpack128x16 (unpack16x8 (unpack128x2 a).`1)) (r0,r1,r2,r3,r4,r5,r6,r7)). auto => />. call (nttunpack128_corr_h (unpack16x8 (unpack128x2 a).`1)) => />. auto => />.
+do 8!(try split; first by
+ apply W16u16.wordP => i Hi; rewrite bits16_W16u16 // Hi //=; rewrite /get256_direct bits16_W32u8 Hi //=; rewrite unpack16x8E unpack128x2E //=; move :Hi; rewrite rng_iotared;
+ do 16!(try (move => Hi; case Hi => />); first by rewrite !initiE //= pack2_bits8 //)).
+seq 8 : ((unpack128x2 rp).`2 = (unpack128x2 a).`2 /\ (unpack128x2 rp).`1 = (unpack128x2 (nttunpack a)).`1 ).
+wp. skip => /> &m -> -> -> -> -> -> -> ->. rewrite nttunpack128x2. rewrite !unpack128x2E => />. split.
++ rewrite tP => j Hj. rewrite !initiE //=. rewrite !initiE //= 1:/#. rewrite !list_arr16 /=.
+  do 8!(rewrite set256_directE 1:/#; rewrite get16_set256E //=; rewrite ifF 1:/#; rewrite get16_init16 1:/#; try(rewrite !initiE //=1:/#)). trivial.
++ rewrite tP => j Hj. rewrite !initiE //= 1:/#. rewrite !list_arr16.
+  do 7!(rewrite set256_directE 1:/#; rewrite get16_set256E //=; rewrite get16_init16 1:/#; rewrite initiE //= 1:/#).
+  rewrite set256_directE 1:/#. rewrite get16_set256E //=. rewrite get16_init16 1:/#. 
+  rewrite !bits16_W16u16. rewrite !unpack16x8K. rewrite !of_listE !initE //= /to_list !nth_mkseq_if //=. rewrite rng_perm_nttunpack128 //=. rewrite !unpack16x8E //=. rewrite !initE //=. rewrite /nttunpack128 !initE //=. rewrite !initE //=. rewrite !rng_perm_nttunpack128 //=. smt().
+sp. 
+seq 1 : ((unpack128x2 rp).`2 = (unpack128x2 a).`2 /\ (unpack128x2 rp).`1 = (unpack128x2 (nttunpack a)).`1 /\ is16u16x8 (nttunpack128x16 (unpack16x8 (unpack128x2 a).`2)) (r0,r1,r2,r3,r4,r5,r6,r7)). auto => />. call (nttunpack128_corr_h (unpack16x8 (unpack128x2 a).`2)) => />. auto => /> &m <- H2.
+do 8!(try split; first by
+ apply W16u16.wordP => i Hi; rewrite bits16_W16u16 // Hi //=; rewrite /get256_direct bits16_W32u8 Hi //=; rewrite unpack16x8E unpack128x2E //=; move :Hi; rewrite rng_iotared => />;
+ do 16!(try (move => Hi; case Hi => />); first by rewrite !initiE //= pack2_bits8 //)).
+auto => /> &m H1 H2 -> -> -> -> -> -> -> ->.
+apply inj_unpack128x2 => />. rewrite -(unpack128x2K rp{m}) (prod (unpack128x2 rp{m})). rewrite (prod (unpack128x2 (nttunpack a))). 
+move :H1 H2. move => -> ->.
+rewrite nttunpack128x2 !unpack16x8K !list_arr16 !unpack128x2E !pack128x2E => />. split.
++ rewrite tP => i Hi.
+  rewrite !initiE //= 1:/#. rewrite !initiE //=. rewrite rng_perm_nttunpack128 //.
+  do 8!(rewrite set256_directE 1:/# get16_set256E //=; rewrite ifF 1:/#; rewrite get16_init16 1:/#; rewrite !initiE //= 1:/#).
+  rewrite ifT //=. rewrite /nttunpack128 !initiE //= 1:/#. rewrite !initiE //=. rewrite rng_perm_nttunpack128 1:/#. smt().
++ rewrite tP => i Hi. rewrite !initiE //=. rewrite !initiE //= 1:/#. rewrite rng_perm_nttunpack128 //.
+  do 8!(rewrite set256_directE 1:/# get16_set256E //=; rewrite get16_init16 1:/#; rewrite !initiE //= 1:/#).
+  rewrite !bits16_W16u16. rewrite !of_listE !initE //= /to_list !nth_mkseq_if //=. rewrite !unpack16x8E //=. rewrite !initE //=. rewrite /nttunpack128 !initE //=. rewrite !initE //=. rewrite !rng_perm_nttunpack128 //= 1..2:/#.
+qed.
+
+lemma _nttunpack_ll: islossless Jkem_avx2.M(Jkem_avx2.Syscall)._nttunpack by islossless.
+
+phoare nttunpack_corr a :
+ [ Jkem_avx2.M(Jkem_avx2.Syscall)._nttunpack : arg = a ==> res = nttunpack a] = 1%r.
+conseq _nttunpack_ll (nttunpack_corr_h a) => />. qed.
+
+
+
+lemma lift768_nttunpack (v : W16.t Array768.t):
+  lift_array768 (nttunpackv v) = nttunpackv (lift_array768 v).
+rewrite /lift_array768 /nttunpackv tP => k kb.
+rewrite mapiE //= !initiE //=.
+case (0<=k <256).
++ move => *; rewrite /subarray256 /nttunpack !initiE //=.
+  pose a:=nttunpack_idx.[k].
+  rewrite initiE //=. smt(nttunpack_bnd Array256.allP).
+  rewrite initiE //=. smt(nttunpack_bnd Array256.allP).
+  rewrite mapiE //=. smt(nttunpack_bnd Array256.allP).
+case (256<=k <512).
++ move => *; rewrite /subarray256 /nttunpack !initiE //=. smt(). smt().
+  pose a:=nttunpack_idx.[k-256].
+  rewrite initiE //=. smt(nttunpack_bnd Array256.allP).
+  rewrite initiE //=. smt(nttunpack_bnd Array256.allP).
+  rewrite mapiE //=. smt(nttunpack_bnd Array256.allP).
+move => *; rewrite /subarray256 /nttunpack !initiE //=. smt(). smt().
+pose a:=nttunpack_idx.[k-512].
+rewrite initiE //=. smt(nttunpack_bnd Array256.allP).
+rewrite initiE //=. smt(nttunpack_bnd Array256.allP).
+rewrite mapiE //=. smt(nttunpack_bnd Array256.allP).
+qed.
+(********************************************************)
+
 
 module HmoduleLow = {
    proc __gen_matrix(sd : W8.t Array32.t, trans : bool) : W16.t Array2304.t = {
@@ -74,11 +322,8 @@ rcondt 1;1: by auto.
 call (sampleAT_sem _sd);auto => />.
 qed.
 
-phoare nttunpack_corr a :
- [ Jkem_avx2.M(Jkem_avx2.Syscall)._nttunpack : arg = a ==> res = nttunpack a] = 1%r.
-admitted. (* proved in indcpa *)
 
-timeout 1.
+op unlift_polyu(a : poly) = Array256.init (fun i => W16.of_int (Zq.asint a.[i])).
 
 lemma sampleA_pos r c _sd b:
   0 <= r < 3 =>
@@ -86,14 +331,19 @@ lemma sampleA_pos r c _sd b:
   subarray256
     (subarray768
        (unlift_matrix (if b then sampleA _sd else sampleA _sd)) r) c = 
-     unlift_poly ((if b then sampleA _sd else sampleA _sd).[r,c])%PolyMat.
-admitted.
+     unlift_polyu ((if b then sampleA _sd else sampleA _sd).[r,c])%PolyMat.
+move => rb cb.
+rewrite /subarray256 /unlift_poly tP => k kb.
+rewrite !Array256.initiE 1,2:/# /= /subarray768 Array768.initiE 1:/# /=.
+rewrite /unlift_matrix Array2304.initiE 1:/# /= getmE /=.
+smt().
+qed.
 
 phoare sample_last _rho :
  [ Jkem_avx2.M(Jkem_avx2.Syscall).__gen_matrix_sample_one_polynomial :
    rho = _rho /\ rc = W16.of_int (2*256+2) ==> 
    res.`1 = subarray256 (subarray768 (unlift_matrix (sampleA _rho)) 2) 2 ] = 1%r.
-have -> : subarray256 (subarray768 (unlift_matrix (sampleA _rho)) 2) 2 = unlift_poly (parse (SHAKE128_ABSORB_34 _rho ((of_int 2))%W8 ((W8.of_int 2)))).`1.
+have -> : subarray256 (subarray768 (unlift_matrix (sampleA _rho)) 2) 2 = unlift_polyu (parse (SHAKE128_ABSORB_34 _rho ((of_int 2))%W8 ((W8.of_int 2)))).`1.
 +  have //=  -> := sampleA_pos 2 2 _rho false _ _ => //.
    by rewrite /sampleA /=;congr; rewrite setmE getmE /= offunmE /#. 
 proc => /=.
